Handle prefix, suffix, and substring.

parser/StringLemmas.fst
@@ -4,12 +4,20 @@ open FStar.String
 open FStar.List.Tot
 open FStar.Classical
      
-// Need to define substrings to state that the parser consumes
+// Need to define prefixes to state that the parser consumes
 // a portion of the input and leaves the rest.
-let is_substring (a:string) (b:string) : bool = 
-  if strlen a = 0 then true else
+let is_prefix (a:string) (b:string) : bool = 
   if strlen a > strlen b then false else
   (sub b 0 (strlen a)) = a
+
+let is_suffix (a:string) (b:string) : bool = 
+  if strlen a > strlen b then false else
+  (sub b (strlen b - strlen a) (strlen a)) = a
+
+let is_substring (a:string) (b:string) : prop = 
+  exists (i:nat) (n:nat{n+i <=strlen b}) . (sub b i n) == a 
+
+(* Lemmas about sub-lists *)
 
 // First n elmements of a list
 let rec first_n #a (n:nat) (l:(list a){length l >= n}) : (x:(list a){length x = n}) =
@@ -32,14 +40,30 @@ let rec sublist_of_whole_length #a (l:(list a)) :
    | [] -> ()
    | hd ::tl -> sublist_of_whole_length tl
 
-// Taking a sublist of a sublist gives the shorter sublist
-let rec sublist_of_sublist_is_sublist #a (l:(list a)) (x:nat{length l >= x}) (y:nat{y <= x}) 
+// Taking a prefix of a prefix gives the shorter prefix
+let rec prefix_of_prefix_of_sublist #a (l:(list a)) (x:nat{length l >= x}) (y:nat{y <= x}) 
  : Lemma (ensures (sublist 0 y l) == (sublist 0 y (sublist 0 x l)))
   = if y = 0 then ()
     else match l with
-    hd :: tl -> sublist_of_sublist_is_sublist tl (x-1) (y-1)
-    
-// String lemmas: have to admit because no model exists, and 
+    hd :: tl -> prefix_of_prefix_of_sublist tl (x-1) (y-1)
+
+// Taking a sublist of the sublist gives a particular sublist
+let rec sublist_of_sublist_is_sublist #a (l:(list a)) 
+   (p1:nat) (n1:nat{p1+n1 <= length l})  // a sublist
+   (p2:nat) (n2:nat{p2+n2 <= n1})        // a sublist of that
+ : Lemma (ensures (sublist p2 n2 (sublist p1 n1 l)) 
+                == (sublist (p1+p2) n2 l))
+  = if p1 = 0 then
+      if p2 = 0 then
+         prefix_of_prefix_of_sublist l n1 n2
+      else
+         match l with
+           hd :: tl -> sublist_of_sublist_is_sublist tl 0 (n1-1) (p2-1) n2
+    else match l with
+      hd :: tl -> sublist_of_sublist_is_sublist tl (p1-1) n1 p2 n2
+
+
+// String lemmas: have to admit this definition because no model exists, and 
 // standard library lemmas are not strong enough; they don't state anything
 // about sub.
 // This is my attempt to define sub in terms of things that *are* strong enough
@@ -48,6 +72,16 @@ let substring_is_sublist (s:string) (i:nat) (l:nat{i+l <= strlen s}) :
   Lemma (ensures (sub s i l) =
                  (string_of_list (sublist i l (list_of_string s))))
      = admit()
+
+let prefix_is_substring (a:string) (b:string) 
+  : Lemma (requires (is_prefix a b))
+          (ensures (is_substring a b))
+  = ()
+
+let suffix_is_substring (a:string) (b:string) 
+  : Lemma (requires (is_suffix a b))
+          (ensures (is_substring a b))
+  = ()
 
 // Derived lemmas
 let all_strings_of_length_zero_are_equal (s:string{strlen s=0}) (t:string{strlen t=0}) 
@@ -64,18 +98,36 @@ let substring_of_length_is_equal (s:string)
      // assert( sublist 0 (strlen s) (list_of_string s) = (list_of_string s) );
      string_of_list_of_string s
 
+let prefix_is_reflexive (s:string)
+ : Lemma (ensures is_prefix s s)
+   = substring_of_length_is_equal s
+
+let suffix_is_reflexive (s:string)
+ : Lemma (ensures is_suffix s s)
+   = substring_of_length_is_equal s
+
 let substring_is_reflexive (s:string)
  : Lemma (ensures is_substring s s)
    = substring_of_length_is_equal s
+
+let prefix_is_shorter (a:string) (b:string) 
+ : Lemma (requires (is_prefix a b))
+         (ensures (strlen a) <= (strlen b) )
+   = ()
+
+let suffix_is_shorter (a:string) (b:string) 
+ : Lemma (requires (is_suffix a b))
+         (ensures (strlen a) <= (strlen b) )
+   = ()
 
 let substring_is_shorter (a:string) (b:string) 
  : Lemma (requires (is_substring a b))
          (ensures (strlen a) <= (strlen b) )
    = ()
 
-let substring_of_substring_is_substring (s:string) (x:nat{strlen s >= x}) (y:nat{y <= x})
+let prefix_of_prefix_is_prefix (s:string) (x:nat{strlen s >= x}) (y:nat{y <= x})
  : Lemma (ensures (sub s 0 y) == (sub (sub s 0 x) 0 y))
- = sublist_of_sublist_is_sublist (list_of_string s) x y;
+ = sublist_of_sublist_is_sublist (list_of_string s) 0 x 0 y;
    //     (sublist 0 y (list_of_string s))
    // ==  (sublist 0 y (sublist 0 x (list_of_string s)))
    // therefore 
@@ -90,16 +142,40 @@ let substring_of_substring_is_substring (s:string) (x:nat{strlen s >= x}) (y:nat
    // Then simplify to (sub s 0 y) == (sub XXXXXXX o y)
    substring_is_sublist (string_of_list (sublist 0 x (list_of_string s))) 0 y;
    substring_is_sublist s 0 x
-   
-// Lemma: a substring of a substring is a substring
-let substring_transitivity (a:string) (b:string) (c:string) :
-  Lemma (requires (is_substring a b) /\ (is_substring b c))
-        (ensures (is_substring a c)) 
+
+// TODO: prove via duality instead?
+// Same plan as above
+let suffix_of_suffix_is_suffix (s:string) (x:nat{strlen s >= x}) (y:nat{y <= x})
+ : Lemma (ensures (suffix s y) == (suffix (suffix s x) y))
+ = sublist_of_sublist_is_sublist (list_of_string s) (strlen s - x) x (x - y) y;
+   substring_is_sublist s (strlen s - x + x - y) y;
+   assert( (sub s (strlen s - y) y) == string_of_list (sublist (x-y) y (sublist (strlen s - x) x (list_of_string s))));
+   list_of_string_of_list (sublist (strlen s - x) x (list_of_string s));
+   substring_is_sublist (string_of_list (sublist (strlen s - x) x (list_of_string s))) (x-y) y;
+   substring_is_sublist s (strlen s - x) x
+
+// Lemma: a prefix of a prefix is a prefix
+let prefix_transitivity (a:string) (b:string) (c:string) :
+  Lemma (requires (is_prefix a b) /\ (is_prefix b c))
+        (ensures (is_prefix a c)) 
        // (sub c 0 (strlen b)) = b
        // (sub b 0 (strlen a)) = a     
        // WTP: (sub c 0 (strlen a)) = a
-     = substring_is_shorter a b;  // (strlen a) <= (strlen b)
-       substring_of_substring_is_substring c (strlen b) (strlen a)
+     = prefix_is_shorter a b;  // (strlen a) <= (strlen b)
+       prefix_of_prefix_is_prefix c (strlen b) (strlen a)
+
+let suffix_transitivity (a:string) (b:string) (c:string) :
+  Lemma (requires (is_suffix a b) /\ (is_suffix b c))
+        (ensures (is_suffix a c)) 
+     = suffix_is_shorter a b;
+       suffix_of_suffix_is_suffix c (strlen b) (strlen a)
+
+let substring_transitivity (a:string) (b:string) (c:string) :
+  Lemma (requires (is_substring a b) /\ (is_substring b c))
+        (ensures (is_substring a c)) 
+  = admit()
+// TODO
+
        
 // Lemma if a and b are the same length, then if a is a substring of b,
 // they must be equal.
